CpcMini/SmtEval.lean
@@ -63,6 +63,9 @@ def native_mk_rational : native_Int -> native_Int -> native_Rat
 def native_streq : native_String -> native_String -> native_Bool
   | x, y => decide (x = y)
 
+def native_nat_to_int (x : native_Nat) : native_Int :=
+  (Int.ofNat x)
+
 syntax "native_nat_zero" : term
 macro_rules
   | `(native_nat_zero) => `(Nat.zero)
